

WIDSML From ScratchW-1

3.1 $w = A^{-1}B$

$$w = \begin{bmatrix} \frac{3}{11} & \frac{-1}{11} \\ \frac{-1}{11} & \frac{4}{11} \end{bmatrix} \begin{bmatrix} 1 \\ 2 \end{bmatrix}$$

$$= \begin{bmatrix} \frac{1}{11} \\ \frac{7}{11} \end{bmatrix}$$

$$Aw = \begin{bmatrix} 4 & 1 \\ 1 & 3 \end{bmatrix} \begin{bmatrix} \frac{1}{11} \\ \frac{7}{11} \end{bmatrix} = \begin{bmatrix} 1 \\ 2 \end{bmatrix} = b$$

$R_2 - 4R_1 \rightarrow 4$

$$\begin{array}{cc|cc} 4 & 1 & 1 & 0 \\ 0 & \frac{11}{4} & -\frac{1}{4} & 1 \end{array}$$

$3 - \frac{1}{4}$

$\downarrow R_1 - \frac{4}{11}R_2$

$$\begin{array}{cc|cc} 4 & 0 & \frac{12}{11} & -\frac{4}{11} \\ 0 & \frac{11}{4} & -\frac{1}{4} & 1 \end{array}$$

$1 + \frac{4}{11} \times \frac{1}{4}$

$\downarrow R_1 \times \frac{1}{4}, R_2 \times \frac{4}{11}$

$$\begin{array}{cc|cc} 1 & 0 & \frac{3}{11} & -\frac{1}{11} \\ 0 & 1 & -\frac{1}{11} & \frac{4}{11} \end{array}$$

3.2

1. $\frac{df}{dx} = 2x + 3$

2. $\frac{\partial g}{\partial x_1} = 2x_1 + 2x_2$

$\frac{\partial g}{\partial x_2} = 2x_1 + 6x_2$

3. $\frac{dh}{dx} = \begin{bmatrix} 2x \\ 3 \end{bmatrix}$

Notes

Date / /

$$4. \nabla_x g = \begin{bmatrix} \frac{\partial g}{\partial x_1} \\ \frac{\partial g}{\partial x_2} \end{bmatrix} = \begin{bmatrix} 2x_1 + 2x_2 \\ 2x_1 + 6x_2 \end{bmatrix}$$

$$5. g(x_1, x_2) = x^T A x$$

$$\begin{bmatrix} a & b \\ c & d \end{bmatrix}$$

$$g(x_1, x_2) = x_1^2 + 2x_1x_2 + 3x_2^2$$

$$= [x_1 \ x_2] \begin{bmatrix} a & b \\ c & d \end{bmatrix} \begin{bmatrix} x_1 \\ x_2 \end{bmatrix}$$

$$= [ax_1 + cx_2 \quad bx_1 + dx_2] \begin{bmatrix} x_1 \\ x_2 \end{bmatrix}$$

$$ax_1^2 + (b+c)x_1x_2 + dx_2^2$$

$$a=1$$

$$d=3$$

$$b+c=2$$

$$b=c \Rightarrow b=1$$

$$A = \begin{bmatrix} 1 & 1 \\ 1 & 3 \end{bmatrix}$$

$$6. \frac{\partial}{\partial x} (x^T A x) = \frac{\partial}{\partial x} (g(x_1, x_2)) = \begin{bmatrix} 2x_1 + 2x_2 \\ 2x_1 + 6x_2 \end{bmatrix}$$

$$p(x_1, x_2) = \begin{bmatrix} 2x_1 + 2x_2 \\ 2x_1 + 6x_2 \end{bmatrix}$$

$$\begin{bmatrix} 2 & 2 \\ 2 & 6 \end{bmatrix} = p = 2A$$

Notes

$$\sum_{i=1}^n (A^T x)_i$$

$$(a) \sum_{i=1}^n$$

$$\sum_{i=1}^n \left(\begin{bmatrix} a & c \\ b & d \end{bmatrix} \begin{bmatrix} x_1 \\ x_2 \end{bmatrix} \right) = \begin{bmatrix} ax_1 + cx_2 \\ bx_1 + dx_2 \end{bmatrix}$$

$$A = \begin{bmatrix} a & b \\ c & d \end{bmatrix}$$

(column
row vector)

$$A = \begin{bmatrix} a_1 \\ \vdots \\ a_n \end{bmatrix}$$

$$A^T x = \sum_{i=1}^n a_i x_i$$

$$A^T = \text{row vector}$$

$$\sum_{i=1}^n (A^T x)_i = a_i$$

$$A^T (a_1, a_2, \dots, a_n)$$

$$= \begin{bmatrix} a_1 \\ a_2 \\ a_3 \\ \vdots \\ a_n \end{bmatrix} = A$$

$$4.1 \quad P(D|+) = \frac{P(+|D)P(D)}{P(+|D)P(D) + P(+|\bar{D})P(\bar{D})}$$

$$= \frac{0.99 \times 0.01}{0.99 \times 0.01 + 0.05 \times 0.99}$$

$$P(\bar{D}) = 0.99$$

$$P(+|\bar{D}) = 0.99 \times 0.01 + 0.05 \times 0.99$$

$$= \frac{99}{99 + 495} = \frac{99}{594} = 0.1666$$

4.2

$$L(\mu, \sigma^2) = p(x_1, x_2, \dots, x_n | \mu, \sigma^2) = \prod_{i=1}^n p(x_i | \mu, \sigma^2)$$

Independent & identically distributed

$$p(x_i^0 | \mu, \sigma^2) = \frac{1}{\sqrt{2\pi\sigma^2}} \exp\left(-\frac{(x_i^0 - \mu)^2}{2\sigma^2}\right)$$

$$L(\mu, \sigma^2) = \prod_{i=1}^n \frac{1}{\sqrt{2\pi\sigma^2}} \exp\left(-\frac{(x_i^0 - \mu)^2}{2\sigma^2}\right)$$

$$= \frac{1}{(\sqrt{2\pi\sigma^2})^n} \exp\left[-\frac{1}{2\sigma^2} \sum_{i=1}^n (x_i^0 - \mu)^2\right]$$

$$\begin{aligned} 2. \quad l(\mu, \sigma^2) &= \ln(L(\mu, \sigma^2)) \\ &= \ln\left[\frac{1}{(\sqrt{2\pi\sigma^2})^n} \exp\left(-\frac{1}{2\sigma^2} \sum_{i=1}^n (x_i^0 - \mu)^2\right)\right] \\ &= n \ln\left(\frac{1}{\sqrt{2\pi\sigma^2}}\right) - \frac{1}{2\sigma^2} \sum_{i=1}^n (x_i^0 - \mu)^2 \\ &= n \ln(2\pi\sigma^2)^{-\frac{1}{2}} - \frac{1}{2\sigma^2} \sum_{i=1}^n (x_i^0 - \mu)^2 \\ &= -\frac{n}{2} \ln(2\pi\sigma^2) - \frac{1}{2\sigma^2} \sum_{i=1}^n (x_i^0 - \mu)^2 \end{aligned}$$

$$\begin{aligned} 3. \quad \frac{\partial}{\partial \mu} (l) &= -\frac{1}{2\sigma^2} \sum_{i=1}^n 2(x_i^0 - \mu) = -\frac{1}{\sigma^2} \sum_{i=1}^n (x_i^0 - \mu) \\ &= \frac{\sum_{i=1}^n x_i^0}{\sigma^2} - \frac{n\mu}{\sigma^2} \end{aligned}$$

$$\frac{\sum_{i=1}^n x_i^0}{n} = \mu = \text{Mean}$$

$$= 0$$

Notes

$$4. \frac{\partial}{\partial \sigma^2} (l) = \frac{-n \times 2\pi}{2 \times 2\pi \sigma^2} + \frac{1}{2\sigma^4} \sum_{i=1}^n (x_i^0 - \mu)^2$$

$$= \frac{-n \times 2\pi}{4\pi \sigma^2} + \frac{1}{2\sigma^4} \sum_{i=1}^n (x_i^0 - \mu)^2 = 0$$

$$\frac{1}{2\sigma^4} \sum_{i=1}^n (x_i^0 - \mu)^2 + \frac{n \times 2\pi}{4\pi \sigma^2} = 0 \Rightarrow \sigma^2 = \frac{\sum_{i=1}^n (x_i^0 - \mu)^2}{n}$$

$$= \text{Variance}$$

$$5. \hat{\mu}_{MLE} = \frac{\sum_{i=1}^n x_i^0}{n} \quad \hat{\sigma}_{MLE}^2 = \frac{\sum_{i=1}^n (x_i^0 - \hat{\mu}_{MLE})^2}{n}$$

5.

1. 10

2. Simple function $f(x) = 2x$

$$3. \begin{aligned} 8a + 4b + 2c + d &= 4 & 16a + 8b &= 64a + 16b \\ 64a + 16b + 4c + d &= 8 & 48a + 8b &= 0 \\ 72a + 8b + 9c + d &= 18 & -6a &= b \end{aligned}$$

$$4 = 48a + 8b + 56a + 12b + 2c = 4 \quad 28a + 6b + c = 2$$

$$665a + 65b + 5c = 10 \Rightarrow 133a + 13b + c = 2$$

$$28a - 90a + c = 2$$

$$28a + 6b + c = 133a + 13b + c$$

$$-62a + c = 2$$

$$7b + 105a = 0$$

$$b = -15a$$

$$133a - 195a + c = 2 \Rightarrow$$

$$c = 2 + 62a$$

Notes

Date / /

$$56a + 12(-15a) + 2(2+62a) = 4 \Rightarrow 56a + 124a - 180a + 4 = 4$$

$$8a + 4(-15a) + 2(2+62a) + d = 4$$

$$(8 - 60 + 124)a + 4 + d = 4 \quad 72a + d = 0$$

$$d = -72a$$

$$f(5) = a(125) - 15a(25) + (2+62a)5 - 72a$$

$$= (125 - 375 + 310 - 72)a + 10$$

$$= 435 - 447a + 10$$

$$= -12a + 10$$

Need not be 10, only if $a=0$

4. Assumption that the relationship is linear

5. The hypothesis used in linear regression is that is null hypothesis and its opposite, alternate hypothesis. If the model is

$$y = \hat{\beta}_0 + \hat{\beta}_1 x$$

Null hypothesis is the case when $\hat{\beta}_1 = 0$, implying no relation between x and y , and in alternate hypothesis, $\hat{\beta}_1 \neq 0$

If the standard error of $\hat{\beta}_1$ is less and $\hat{\beta}_1$ is large, then the null hypothesis can be

ignored. $t\text{-statistic} = \frac{\hat{\beta}_1 - 0}{SE(\hat{\beta}_1)}$

~~t ↑~~ ⇒ ~~Alter~~

p-value is the probability of how much the null hypothesis condition holds good.
Lower p-value, means relationship exists.

If p value is not very small, and greater than 1%, null hypothesis can be ~~rejected~~ confirmed.

6. If there are d features

$$y = \hat{\beta}_0 + \hat{\beta}_1 x_1 + \dots + \hat{\beta}_d x_d$$

For each x_i ($i \in [1, d]$), there is an associated with t-statistic and p-value.

If the p-value is sufficiently large for any particular x_i , we can confirm null hypothesis and remove that feature's contribution to y .

9. Considering data points $(x_1, y_1), (x_2, y_2), \dots, (x_n, y_n)$, loss for each term = $(y_i - \hat{y}_i)^2$ (squared)

total $\hat{y} = wx + b$

$$L = \text{total loss} = \sum_{i=1}^n (y_i^0 - \hat{y}_i)^2 = \sum_{i=1}^n (y_i^0 - (wx_i^0 + b))^2$$

$$10. \frac{\partial L}{\partial w} = \sum_{i=1}^n 2(y_i^0 - (wx_i^0 + b))(-x_i^0)$$

$$= \sum_{i=1}^n 2x_i^0 (wx_i^0 + b - y_i^0) = 0$$

$$= \sum_{i=1}^n x_i^0 (\cancel{wx_i^0 + b} - y_i^0) (y_i^0 - (wx_i^0 + b)) = 0$$

$$\frac{\partial L}{\partial b} = \sum_{i=1}^n 2(y_i^0 - (wx_i^0 + b))(-1) = 0$$

$$= \sum_{i=1}^n (y_i^0 - (wx_i^0 + b)) = 0$$

$$\Rightarrow \sum_{i=1}^n y_i^0 - w \sum_{i=1}^n x_i^0 - nb = 0$$

$$\sum y_i^0 = w \sum x_i^0 + nb$$

$$\frac{\sum y_i^0}{n} = w \frac{\sum x_i^0}{n} + b$$

$$\bar{y} = w\bar{x} + b$$

$$b = \bar{y} - w\bar{x}$$

$$\sum x_i^0 y_i^0 - \omega \sum x_i^0{}^2 + b \sum x_i^0 = 0$$

$$\sum x_i^0 y_i^0 - \omega \sum x_i^0{}^2 + (\bar{y} - \omega \bar{x}) \sum x_i^0 = 0$$

$$\sum x_i^0 (y_i^0 - \omega x_i^0 - \bar{y} + \omega \bar{x}) = 0$$

$$= \sum x_i^0 ((y_i^0 - \bar{y}) - \omega (x_i^0 - \bar{x})) = 0$$

$$\sum x_i^0 (y_i^0 - \bar{y}) - \omega \sum x_i^0 (x_i^0 - \bar{x}) = 0$$

$$\omega = \frac{\sum x_i^0 (y_i^0 - \bar{y})}{\sum x_i^0 (x_i^0 - \bar{x})} = \frac{\sum x_i^0 y_i^0 - \bar{y} \sum x_i^0}{\sum x_i^0{}^2 - \bar{x} \sum x_i^0}$$

$$\bar{y} = \frac{\sum y_i^0}{n} \Rightarrow \sum y_i^0 = n \bar{y}$$

$$\omega = \frac{n \bar{x} (\sum (y_i^0 - \bar{y}))}{n \bar{x} \sum (x_i^0 - \bar{x})}$$

$$\omega = \frac{\sum x_i^0 y_i^0 - \bar{y} \sum x_i^0}{\sum x_i^0{}^2 - \bar{x} \sum x_i^0}$$

$$= \frac{\sum x_i^0 y_i^0 - \bar{y} n \bar{x}}{\sum x_i^0{}^2 - \bar{x} n \bar{x}} = \frac{\sum x_i^0 y_i^0 - n \bar{x} \bar{y}}{\sum x_i^0{}^2 - \bar{x}^2 n}$$

$$\begin{aligned} \sum (x_i^0 - \bar{x})^2 &= \sum (x_i^0{}^2 + \bar{x}^2 - 2x_i^0 \bar{x}) \\ &= \sum x_i^0{}^2 - n \bar{x}^2 - 2\bar{x} \sum x_i^0 \\ &= \sum x_i^0{}^2 + n \bar{x}^2 - 2\bar{x} n \bar{x} \\ &= \sum x_i^0{}^2 - n \bar{x}^2 \end{aligned}$$

$$\begin{aligned} \sum x_i^0 (y_i^0 - \bar{y}) &= \sum x_i^0 y_i^0 - \bar{y} \sum x_i^0 \\ &= \sum x_i^0 y_i^0 - n \bar{x} \bar{y} \end{aligned}$$

$$\sum x_i^0 y_i^0 - n \bar{x} \bar{y}$$

$$\begin{aligned} &= \sum x_i^0 y_i^0 \\ &\quad - \bar{x} \sum y_i^0 \\ &\quad - \bar{y} \sum x_i^0 \\ &\quad + n \bar{x} \bar{y} \end{aligned}$$

$$\frac{\sum x_i^0 (y_i^0 - \bar{y})}{\sum x_i^0 (x_i^0 - \bar{x})} = \frac{\sum (x_i^0 - \bar{x}) (y_i^0 - \bar{y})}{\sum (x_i^0 - \bar{x})^2} = w$$

$$11. \hat{y} = wX \quad w = \begin{bmatrix} b \\ w_1 \\ w_2 \\ \vdots \\ w_d \end{bmatrix}$$

$$12. L = \|y - \hat{y}\|^2 = \|y - Xw\|^2$$

$\|a\|^2$ $a \Rightarrow$ column vector

$$\|a\|^2 = a^T a \begin{bmatrix} a_1 & a_2 & \dots \end{bmatrix} \begin{bmatrix} a_1 \\ a_2 \\ \vdots \end{bmatrix} = \begin{bmatrix} a_1 & a_2 & \dots \end{bmatrix} \begin{bmatrix} a_1^2 + a_2^2 + \dots \end{bmatrix} = \|a\|^2$$

$$L = (y - Xw)^T (y - Xw)$$

$$13. L = \cancel{(y - Xw)^T} (y - Xw) = (y^T - X^T w^T) (y - Xw)$$

$$= \cancel{y^T y - X^T w^T y - y^T X w + X^T w^T X w}$$

$$= (y - Xw)^T (y - Xw) = (y^T - w^T X^T) (y - Xw)$$

$$= y^T y - w^T X^T y - y^T X w + w^T X^T X w$$

$$[b \ w_1 \ \dots \ w_d] \begin{bmatrix} x_1 \\ \vdots \\ x_{nd} \end{bmatrix}$$

$$\left[\begin{array}{c|c} \dots & d \\ \hline d & \dots \end{array} \right] \begin{bmatrix} \vdots \\ d \end{bmatrix} = \text{Scalar}$$

$$(w^T x^T y)^T = \cancel{w x y^T} \quad \cancel{y^T w} y^T w x$$

$$L = y^T y - 2w^T x^T y + w^T x^T w x$$

$$\frac{\delta L}{\delta w} = -2x^T y + 2x^T x w = 0 \quad (\text{Max Min L})$$

$$2x^T y = 2x^T x w$$

$$\cancel{w} = x^T y = x^T x w$$

$$w = (x^T x)^{-1} x^T y$$